

› § ê

W

-

ê §



~`/fz~(%fz1/

1. Initialization

$\hat{e} = \frac{1}{\sqrt{2}} \begin{bmatrix} 1 \\ 0 \end{bmatrix}$
 $\hat{e} = \frac{1}{\sqrt{2}} \begin{bmatrix} 0 \\ 1 \end{bmatrix}$
 $\hat{e} = \frac{1}{\sqrt{2}} \begin{bmatrix} 1 \\ 1 \end{bmatrix}$
 $\hat{e} = \frac{1}{\sqrt{2}} \begin{bmatrix} 1 \\ -1 \end{bmatrix}$

$j = 1$
 $3 \hat{e} = \frac{1}{\sqrt{2}} \begin{bmatrix} 3 \\ 0 \end{bmatrix}$
 $\hat{e} = \frac{1}{\sqrt{2}} \begin{bmatrix} 1 \\ 0 \end{bmatrix}$
 $\hat{e} = \frac{1}{\sqrt{2}} \begin{bmatrix} 0 \\ 1 \end{bmatrix}$
 $\hat{e} = \frac{1}{\sqrt{2}} \begin{bmatrix} 1 \\ 1 \end{bmatrix}$
 $\hat{e} = \frac{1}{\sqrt{2}} \begin{bmatrix} 1 \\ -1 \end{bmatrix}$

$i = 1$
 $\hat{e} = \frac{1}{\sqrt{2}} \begin{bmatrix} 1 \\ 0 \end{bmatrix}$
 $\hat{e} = \frac{1}{\sqrt{2}} \begin{bmatrix} 0 \\ 1 \end{bmatrix}$
 $\hat{e} = \frac{1}{\sqrt{2}} \begin{bmatrix} 1 \\ 1 \end{bmatrix}$
 $\hat{e} = \frac{1}{\sqrt{2}} \begin{bmatrix} 1 \\ -1 \end{bmatrix}$

$i = 1$
 $\hat{e} = \frac{1}{\sqrt{2}} \begin{bmatrix} 1 \\ 0 \end{bmatrix}$
 $\hat{e} = \frac{1}{\sqrt{2}} \begin{bmatrix} 0 \\ 1 \end{bmatrix}$
 $\hat{e} = \frac{1}{\sqrt{2}} \begin{bmatrix} 1 \\ 1 \end{bmatrix}$
 $\hat{e} = \frac{1}{\sqrt{2}} \begin{bmatrix} 1 \\ -1 \end{bmatrix}$

$\hat{e} = \frac{1}{\sqrt{2}} \begin{bmatrix} 1 \\ 0 \end{bmatrix}$
 $\hat{e} = \frac{1}{\sqrt{2}} \begin{bmatrix} 0 \\ 1 \end{bmatrix}$
 $\hat{e} = \frac{1}{\sqrt{2}} \begin{bmatrix} 1 \\ 1 \end{bmatrix}$
 $\hat{e} = \frac{1}{\sqrt{2}} \begin{bmatrix} 1 \\ -1 \end{bmatrix}$

$3 = 1$

§ -

J i

ê

§ i

ê

i 3 ê

3 ê

3 ê

.

- ê j

-

ê

~ / f~ (% f~ /

- ê

ê ê

§ ê § ê

±

d

~ ê J

, ê

Đ J

§ ê Đ ê Đ , ,

$$j \pm \hat{e}$$

$$- \hat{e} \quad \S$$

$$j \hat{e}$$

$$- \hat{e} \quad \hat{e} \quad \S$$

$$3 \quad j \hat{e}$$

$$- \hat{e} \quad \hat{e} \quad \S$$

$$j \quad \hat{e}$$

$$\hat{e}$$

$$- \hat{e}$$

$$\hat{e}$$

$$> \hat{e}$$

$$\hat{e} \quad , \quad \hat{e} \quad \hat{e}$$

$$\frac{1}{\sqrt{\pi}} \int_{-\infty}^{\infty} e^{-x^2} dx = 1$$

J_u

\hat{e} \hat{e} \hat{e}

$j \quad \hat{e}$
 \hat{e}
 $\hat{e} \hat{e} \quad j \quad \hat{e}-$

3ê J

ê

ê

i ê ĩê

ê

ê

ê

3 i u

ê

i J

ê

ê

ê

3 3 ê

,

3

ê